code/ecdsap256/Hacl.P256.fst
@@ -9,15 +9,78 @@ open Lib.IntTypes
 open Lib.Buffer
 
 open Spec.Hash.Definitions
+open Hacl.Hash.SHA2
 
 open Hacl.Impl.P256.Sign
 open Hacl.Impl.P256.Verify
+
+module LSeq = Lib.Sequence
+module BSeq = Lib.ByteSequence
 
 module S = Spec.P256
 module BN = Hacl.Impl.P256.Bignum
 module P = Hacl.Impl.P256.Point
 
 #set-options "--z3rlimit 30 --fuel 0 --ifuel 0"
+
+inline_for_extraction noextract
+val msg_as_felem:
+    alg:S.hash_alg_ecdsa
+  -> msg_len:size_t{v msg_len >= S.min_input_length alg}
+  -> msg:lbytes msg_len
+  -> res:BN.felem ->
+  Stack unit
+  (requires fun h ->
+    live h msg /\ live h res /\ disjoint msg res)
+  (ensures fun h0 _ h1 -> modifies (loc res) h0 h1 /\
+    (let hashM = S.hash_ecdsa alg (v msg_len) (as_seq h0 msg) in
+    BN.as_nat h1 res = BSeq.nat_from_bytes_be (LSeq.sub hashM 0 32) % S.order))
+
+let msg_as_felem alg msg_len msg res =
+  push_frame ();
+
+  [@inline_let] let sz: size_t =
+    match alg with
+    | S.NoHash -> 32ul
+    | S.Hash a -> Hacl.Hash.Definitions.hash_len a in
+
+  let mHash = create sz (u8 0) in
+
+  begin
+  match alg with
+    | S.NoHash -> copy mHash (sub msg 0ul 32ul)
+    | S.Hash a -> match a with
+      | SHA2_256 -> hash_256 msg msg_len mHash
+      | SHA2_384 -> hash_384 msg msg_len mHash
+      | SHA2_512 -> hash_512 msg msg_len mHash
+  end;
+
+  let mHash32 = sub mHash 0ul 32ul in
+  BN.bn_from_bytes_be4 res mHash32;
+  Hacl.Impl.P256.Scalar.qmod_short res res;
+  pop_frame ()
+
+
+inline_for_extraction noextract
+val ecdsa_signature: alg:S.hash_alg_ecdsa -> ecdsa_sign_p256_st alg
+let ecdsa_signature alg signature msg_len msg private_key nonce =
+  push_frame ();
+  let m_q = BN.create_felem () in
+  msg_as_felem alg msg_len msg m_q;
+  let res = ecdsa_sign_msg_as_qelem signature m_q private_key nonce in
+  pop_frame ();
+  res
+
+
+inline_for_extraction noextract
+val ecdsa_verification: alg:S.hash_alg_ecdsa -> ecdsa_verify_p256_st alg
+let ecdsa_verification alg msg_len msg public_key signature_r signature_s =
+  push_frame ();
+  let m_q = BN.create_felem () in
+  msg_as_felem alg msg_len msg m_q;
+  let res = ecdsa_verify_msg_as_qelem m_q public_key signature_r signature_s in
+  pop_frame ();
+  res
 
 
 let ecdsa_sign_p256_sha2 signature msg_len msg private_key nonce =
